books/kestrel/jvm/ieee-floats-as-bvs.lisp
@@ -60,7 +60,6 @@
 ;; The oracle determines how NaNs are encoded.
 (defund encode-bv-float (k p datum oracle)
   (declare (xargs :guard (and (formatp k p)
-                              (< 1 p)
                               (< 1 (- k p)) ; todo
                               (floating-point-datump k p datum))
                   :guard-hints (("Goal" :in-theory (enable formatp)))))
@@ -75,8 +74,7 @@
                   trailing-significand))))
 
 (defthm bv-floatp-of-encode-bv-float
-  (implies (and (formatp k p)
-                (< 1 p))
+  (implies (formatp k p)
            (bv-floatp k (encode-bv-float k p datum oracle)))
   :hints (("Goal" :in-theory (enable encode-bv-float wfn))))
 
@@ -95,7 +93,6 @@
 ;; Inversion
 (defthm decode-bv-float-of-encode-bv-float
   (implies (and (< 1 (- k p)) ; todo
-                (< 1 p)
                 (floating-point-datump k p datum)
                 (formatp k p))
            (equal (decode-bv-float k p (encode-bv-float k p datum oracle))
